@prefix cep: <http://www.cepler.org/ontology#> .
@prefix rdf: <http://www.w3.org/1999/02/22-rdf-syntax-ns#> .
@prefix rdfs: <http://www.w3.org/2000/01/rdf-schema#> .
@prefix schema: <http://schema.org/> .
@prefix wikibase: <http://wikiba.se/ontology#> .

#Cepler Class: Request
cep:Request rdf:type rdfs:Class .
cep:Request rdfs:label "Request" @en .
cep:Request rdfs:comment "Specifies the parameters that are requested, consisting of an input value and an input unit." @en .

#Cepler Property: request
cep:request rdf:type rdf:Property .
cep:request rdf:label "request" @en .
cep:request rdfs:comment "Relates a Cepler Query to its Cepler Request. " @en .
cep:request rdfs:domain cep:Query .
cep:request rdfs:range cep:Request .

#Cepler Property: factor
cep:factor rdf:type rdf:Property .
cep:factor rdf:label "factor" @en .
cep:factor rdfs:comment "Adds a factor to a Cepler Query to set the requested value and a Cepler Result into a numeric relation." @en .
cep:factor rdfs:domain cep:Query .

#Cepler Class: Query
cep:Query rdf:type rdfs:Class .
cep:Query rdfs:label "Query" @en .
cep:Query rdfs:comment "Is a Query to the Cepler API that combines a Cepler Request with a Cepler Result." @en .

#Cepler Class: Result
cep:Result rdf:type rdfs:Class .
cep:Result rdfs:label "Result" @en .
cep:Result rdfs:comment "Is a Result to a Cepler Query being related to a Cepler request." @en .

#Cepler Property: result
cep:result rdf:type rdf:Property .
cep:result rdf:label "result" @en .
cep:result rdfs:comment "Relates a Cepler Query to its Cepler Result." .
cep:result rdfs:domain cep:Query .
cep:result rdfs:range cep:Result .

#Cepler Property: unit
cep:unit rdf:type rdf:Property .
cep:unit rdf:label "unit" @en .
cep:unit rdfs:comment "Adds a unit. "
cep:unit schema:isSimilarTo wikibase:quantityUnit .

#Cepler Property: uri
cep:uri rdf:type rdf:Property .
cep:uri rdf:label "uri" @en .
cep:uri rdfs:comment "Relates a URI to a Cepler Result." @en .
cep:uri rdfs:domain cep:Result .