@prefix rdf: <http://www.w3.org/1999/02/22-rdf-syntax-ns#> .
@prefix rdfs: <http://www.w3.org/2000/01/rdf-schema#> .
@prefix cep: <http://www.cepler.org/ontology#> .

cep:Request rdf:type rdfs:Class .
cep:Request rdfs:label "Request" @en .
cep:Request rdfs:comment "Specifies the parameters that are requested, consisting of an input value and an input unit." @en .


cep:request rdf:type rdf:Property .
cep:request rdf:label "request" @en .
cep:request rdfs:comment "Relates a Cepler Query to its Cepler Request. " @en .
cep:request rdfs:domain cep:Query .
cep:request rdfs:range cep:Request .


cep:factor rdf:type rdf:Property .
cep:factor rdf:label "factor" @en .
cep:factor rdfs:comment "Adds a factor to a Cepler Query to set the requested value and a Cepler Result into a numeric relation." @en .
cep:factor rdfs:domain cep:Query .


cep:Query rdf:type rdfs:Class .
cep:Query rdfs:label "Query" @en .
cep:Query rdfs:comment "Is a Query to the Cepler API that combines a Cepler Request with a Cepler Result." @en .


cep:Result rdf:type rdfs:Class .
cep:Result rdfs:label "Result" @en .
cep:Result rdfs:comment "Is a Result to a Cepler Query being related to a Cepler request." @en .


cep:result rdf:type rdf:Property .
cep:result rdf:label "result" @en .
cep:result rdfs:comment "Relates a Cepler Query to its Cepler Result." .
cep:result rdfs:domain cep:Query .
cep:result rdfs:range cep:Result .


cep:unit rdf:type rdf:Property .
cep:unit rdf:label "unit" @en .
cep:unit rdfs:comment "Provides a unit to "


cep:result